adding lemma triggers, fleshing out admits

src/Pipit.Context.fst
@@ -5,11 +5,11 @@ module List = FStar.List.Tot
 
 
 type var (t: Type) =
-  (* Keep constructor so "var int" is different from "var string" ? *)
+  (* Keep constructor so "var int" is different from "var string" *)
   | Var: (v: nat) -> var t
 let index  = nat
 
-(* HACK: AXIOM: assume that all fresh name allocation doesn't reuse names!
+(* AXIOM: assume that all fresh name allocation doesn't reuse names!
    We can't use decidable equality on two variables of different type variables
    (x: var 'a) and (x': var 'b) because equality on Type isn't decidable.
  *)
@@ -43,12 +43,12 @@ let rec lift1 (l: list 'a) (i: nat { i <= List.length l }) (v: 'a): (l': list 'a
   | _, 0 -> v :: l
   | l0 :: l', _ -> l0 :: lift1 l' (i - 1) v
 
-let rec row (l: list Type): Type =
+let rec row (l: context): Type =
   match l with
   | [] -> unit
   | t :: ts -> t * row ts
 
-let rec row_index (l: list Type) (r: row l) (i: index { i < List.length l }): List.index l i =
+let rec row_index (l: context) (r: row l) (i: index { i < List.length l }): get_index l i =
   match l with
   | t :: ts ->
     let r': t * row (List.tl l) = r in
@@ -95,11 +95,11 @@ let rec row_zip2_lift1 (rs: list (row 'c)) (i: nat { i <= List.length 'c }) (vs:
   | [], [] -> []
   | r :: rs, v :: vs -> row_lift1 r i v :: row_zip2_lift1 rs i vs
 
-let index_drop (i limit: index) (drop_by: nat { drop_by <= limit + 1 }): index =
-  if i > limit then i - drop_by else i
+let index_drop (i limit: index): (r: index { (i > limit ==> r = i - 1) /\ (i <= limit ==> r = i )}) =
+  if i > limit then i - 1 else i
 
-let index_lift (i limit: index) (lift_by: nat): index =
-  if i >= limit then i + lift_by else i
+let index_lift (i limit: index): (r: index { (i >= limit ==> r = i + 1) /\ (i < limit ==> r = i) }) =
+  if i >= limit then i + 1 else i
 
 let open1' (c: context) (i: index { has_index c i }): context = drop1 c i
 let open1 (c: context { has_index c 0 }): context = List.tl c
@@ -107,25 +107,27 @@ let open1 (c: context { has_index c 0 }): context = List.tl c
 let close1' (c: context) (t: Type) (i: index { i <= List.length c }): context = lift1 c i t
 let close1 (c: context) (t: Type): context = t :: c
 
-let lemma_drop0 (c: context { List.length c > 0 }) (t: Type):
+(* Properties should only require one implicit unrolling of recursive definitions, and one implicit inversion *)
+#push-options "--fuel 1 --ifuel 1"
+
+let lemma_drop0 (c: context { List.length c > 0 }):
   Lemma (ensures (drop1 c 0 == List.tl c)) = ()
 
 let lemma_lift0 (c: context) (t: Type):
   Lemma (ensures (lift1 c 0 t == t :: c)) = ()
 
+// XXX: these look like good candidates for SMT patterns but seem to cause flakiness
 let lemma_dropCons (c0: Type) (c': context) (i: index { 0 < i /\ i <= List.length c' }):
-  Lemma (ensures (drop1 (c0 :: c') i == c0 :: drop1 c' (i - 1))) = ()
+  Lemma (ensures (drop1 (c0 :: c') i == c0 :: drop1 c' (i - 1)))
+        = // [SMTPat (drop1 (c0 :: c') i)] =
+  ()
 
 let lemma_liftCons (c0: Type) (c': context) (i: index { 0 < i /\ i <= List.length c' + 1}) (t: Type):
-  Lemma (ensures (lift1 (c0 :: c') i t == c0 :: lift1 c' (i - 1) t)) = ()
+  Lemma (ensures (lift1 (c0 :: c') i t == c0 :: lift1 c' (i - 1) t))
+        = // [SMTPat (lift1 (c0 :: c') i t)] =
+  ()
 
-// let lemma_drop_length (c: context) (i: index { has_index c i }):
-//   Lemma (ensures List.length (drop1 c i) == List.length c - 1) = ()
-
-// let lemma_lift_length (c: context) (i: index { has_index c i }) (t: Type):
-//   Lemma (ensures List.length (lift1 c i t) == List.length c + 1) = ()
-
-let rec lemma_open_preserves_opt_index (c: context) (n: index { has_index c n }) (i: index { i <> n }): Lemma (opt_index c i == opt_index (open1' c n) (index_drop i n 1)) =
+let rec lemma_open_preserves_opt_index (c: context) (n: index { has_index c n }) (i: index { i <> n }): Lemma (opt_index c i == opt_index (open1' c n) (index_drop i n)) =
   match c with
   | [] -> ()
   | _ :: c' ->
@@ -133,7 +135,7 @@ let rec lemma_open_preserves_opt_index (c: context) (n: index { has_index c n })
     then lemma_open_preserves_opt_index c' (n - 1) (i - 1)
     else ()
 
-let rec lemma_close_preserves_opt_index (c: context) (t: Type) (n: index { n <= List.length c }) (i: index): Lemma (opt_index c i == opt_index (close1' c t n) (index_lift i n 1)) =
+let rec lemma_close_preserves_opt_index (c: context) (t: Type) (n: index { n <= List.length c }) (i: index): Lemma (opt_index c i == opt_index (close1' c t n) (index_lift i n)) =
   match c with
   | [] -> ()
   | _ :: c' ->
@@ -141,7 +143,8 @@ let rec lemma_close_preserves_opt_index (c: context) (t: Type) (n: index { n <= 
     then lemma_close_preserves_opt_index c' t (n - 1) (i - 1)
     else ()
 
-let rec lemma_close_contains (c: context) (t: Type) (n: index { n <= List.length c }): Lemma (opt_index (close1' c t n) n == Some t) =
+let rec lemma_close_contains (c: context) (t: Type) (n: index { n <= List.length c }): Lemma (opt_index (close1' c t n) n == Some t)
+  [SMTPat (opt_index (close1' c t n) n)] =
   match c with
   | [] -> ()
   | _ :: c' ->
@@ -164,11 +167,9 @@ let rec lemma_lift_lift_commute (c: context) (i1: index { i1 <= List.length c })
   | c0 :: c' ->
     if i2 > 0
     then (lemma_lift_lift_commute c' (i1 - 1) (i2 - 1) t1 t2;
-      // sometimes fails; spell it out
-      assert (lift1 (lift1 c' (i1 - 1) t1) (i2 - 1) t2 == lift1 (lift1 c' (i2 - 1) t2) i1 t1);
-      assert (lift1 (lift1 (c0 :: c') i1 t1) i2 t2 == lift1 (lift1 (c0 :: c') i2 t2) (i1 + 1) t1);
       ())
     else ()
+
 
 let rec lemma_drop_drop_commute (c: context) (i1: index { has_index c i1 }) (i2: index { i1 <= i2 /\ i2 < List.length c - 1 }):
   Lemma (ensures drop1 (drop1 c i1) i2 == drop1 (drop1 c (i2 + 1)) i1) =
@@ -177,14 +178,13 @@ let rec lemma_drop_drop_commute (c: context) (i1: index { has_index c i1 }) (i2:
   | c0 :: c' ->
     if i1 > 0
     then (lemma_drop_drop_commute c' (i1 - 1) (i2 - 1);
-         // TODO true but sometimes fails; spell it out
-         assume (drop1 (drop1 (c0 :: c') i1) i2 == drop1 (drop1 (c0 :: c') (i2 + 1)) i1);
          ())
 
     else ()
 
 let rec lemma_drop_lift_eq (c: context) (i: index { i <= List.length c }) (t: Type):
-  Lemma (ensures drop1 (lift1 c i t) i == c) =
+  Lemma (ensures drop1 (lift1 c i t) i == c)
+    [SMTPat (drop1 (lift1 c i t) i)] =
   match c with
   | [] -> ()
   | _ :: c' ->
@@ -193,7 +193,8 @@ let rec lemma_drop_lift_eq (c: context) (i: index { i <= List.length c }) (t: Ty
     else ()
 
 let rec lemma_lift_drop_eq (c: context) (i: index { i < List.length c }):
-  Lemma (ensures lift1 (drop1 c i) i (get_index c i) == c) =
+  Lemma (ensures lift1 (drop1 c i) i (get_index c i) == c)
+    [SMTPat (lift1 (drop1 c i) i (get_index c i)) ]=
   match c with
   | [] -> ()
   | _ :: c' ->
@@ -214,44 +215,48 @@ let rec lemma_lift_drop_commute_le (c: context) (i1: index { has_index c i1 }) (
       else ()
     else ()
 
-let rec lemma_lift_get_index (c: context) (i: index { i <= List.length c }) (t: Type):
-  Lemma (ensures get_index (lift1 c i t) i == t) =
+let rec lemma_lift_get_index (c: context) (i1: index { i1 <= List.length c }) (i2: index { i2 <= List.length c }) (t2: Type):
+  Lemma (ensures get_index (lift1 c i2 t2) i1 == (if i1 = i2 then t2 else get_index c (index_drop i1 i2)))
+        [SMTPat (get_index (lift1 c i2 t2) i1)] =
   match c with
   | [] -> ()
   | _ :: c' ->
-    if i > 0
-    then lemma_lift_get_index c' (i - 1) t
+    if i1 > 0 && i2 > 0
+    then
+      lemma_lift_get_index c' (i1 - 1) (i2 - 1) t2
     else ()
 
-let rec lemma_lift_get_index_gt (c: context) (i1: index { has_index c i1 }) (i2: index { i2 <= i1 }) (t2: Type):
+let lemma_lift_get_index_eq (c: context) (i: index { i <= List.length c }) (t: Type):
+  Lemma (ensures get_index (lift1 c i t) i == t)
+        [SMTPat (get_index (lift1 c i t) i)] =
+  lemma_lift_get_index c i i t
+
+let lemma_lift_get_index_gt (c: context) (i1: index { has_index c i1 }) (i2: index { i2 <= i1 }) (t2: Type):
   Lemma (ensures get_index (lift1 c i2 t2) (i1 + 1) == get_index c i1) =
+  lemma_lift_get_index c (i1 + 1) i2 t2
+
+// let lemma_lift_get_index_gt (c: context) (i1: index { i1 <= List.length c }) (i2: index { i2 <= i1 /\ i2 <= List.length c }) (t2: Type):
+//   Lemma (ensures get_index (lift1 c i2 t2) i1 == get_index c (i1 - 1)) =
+//   lemma_lift_get_index c i1 i2 t2
+
+let rec lemma_drop_get_index (c: context) (i1: index { has_index c i1 }) (i2: index { i2 < List.length c - 1 }):
+  Lemma (ensures get_index (drop1 c i1) i2 == get_index c (index_lift i2 i1))
+        [SMTPat (get_index (drop1 c i1) i2)] =
   match c with
   | [] -> ()
   | _ :: c' ->
-    if i2 > 0
+    if i1 > 0 && i2 > 0
     then
-      lemma_lift_get_index_gt c' (i1 - 1) (i2 - 1) t2
+      lemma_drop_get_index c' (i1 - 1) (i2 - 1)
     else ()
 
-let rec lemma_drop_get_index_gt (c: context) (i1: index { has_index c i1 }) (i2: index { i1 <= i2 /\ i2 < List.length c - 1 }):
+let lemma_drop_get_index_gt (c: context) (i1: index { has_index c i1 }) (i2: index { i1 <= i2 /\ i2 < List.length c - 1 }):
   Lemma (ensures get_index (drop1 c i1) i2 == get_index c (i2 + 1)) =
-  match c with
-  | [] -> ()
-  | _ :: c' ->
-    if i1 > 0
-    then
-      lemma_drop_get_index_gt c' (i1 - 1) (i2 - 1)
-    else ()
+  lemma_drop_get_index c i1 i2
 
-let rec lemma_drop_get_index_lt (c: context) (i1: index { has_index c i1 }) (i2: index { i2 < i1 /\ i2 < List.length c - 1 }):
+let lemma_drop_get_index_lt (c: context) (i1: index { has_index c i1 }) (i2: index { i2 < i1 /\ i2 < List.length c - 1 }):
   Lemma (ensures get_index (drop1 c i1) i2 == get_index c i2) =
-  match c with
-  | [] -> ()
-  | _ :: c' ->
-    if i2 > 0
-    then
-      lemma_drop_get_index_lt c' (i1 - 1) (i2 - 1)
-    else ()
+  lemma_drop_get_index c i1 i2
 
 let row_lift1_dropped (i: nat { i < List.length 'c }) (r: row (drop1 'c i)) (v: get_index 'c i): row 'c =
   lemma_lift_drop_eq 'c i;
@@ -260,3 +265,42 @@ let row_lift1_dropped (i: nat { i < List.length 'c }) (r: row (drop1 'c i)) (v: 
 let row_zip2_lift1_dropped (i: nat { i < List.length 'c }) (rs: list (row (drop1 'c i))) (vs: list (get_index 'c i) { List.length rs == List.length vs }): (ret: list (row 'c) { List.length ret == List.length rs }) =
   lemma_lift_drop_eq 'c i;
   row_zip2_lift1 rs i vs
+
+let rec lemma_row_index_lift1_eq
+  (r: row 'c)
+  (i: index { i <= List.length 'c })
+  (v: 'a):
+  Lemma (ensures (row_index (lift1 'c i 'a) (row_lift1 r i v) i == v))
+        [SMTPat (row_index (lift1 'c i 'a) (row_lift1 r i v) i)] =
+  match 'c with
+   | [] -> ()
+   | c :: c' ->
+     let r': c & row c' = r in
+     if i = 0
+     then ()
+     else lemma_row_index_lift1_eq (snd r') (i - 1) v
+
+let rec lemma_row_index_lift1
+  (r: row 'c)
+  (i: index { i <= List.length 'c })
+  (i': index { i' <= List.length 'c })
+  (v: 'a):
+  Lemma (ensures (row_index (lift1 'c i 'a) (row_lift1 r i v) i' == (if i = i' then v else (coerce_eq () (row_index 'c r (index_drop i' i))))))
+        [SMTPat (row_index (lift1 'c i 'a) (row_lift1 r i v) i')] =
+  match 'c with
+   | [] -> ()
+   | c :: c' ->
+     let r': c & row c' = r in
+     if i = 0 || i' = 0
+     then ()
+     else lemma_row_index_lift1 (snd r') (i - 1) (i' - 1) v
+
+let rec lemma_row_zip2_lift1_row_zip2_cons
+  (rows: list (row 'c))
+  (vs: list 'a { List.length rows == List.length vs }):
+  Lemma (ensures (row_zip2_lift1 rows 0 vs == row_zip2_cons vs rows))
+        [SMTPat (row_zip2_lift1 rows 0 vs)] =
+  match rows, vs with
+  | [], [] -> ()
+  | _ :: rows', _ :: vs' ->
+    lemma_row_zip2_lift1_row_zip2_cons rows' vs'
